Add Kleene-algebra setoid, refine IMP, prove weak Hoare lemmas

theories/Hoare.v
@@ -1,65 +1,378 @@
-(* Require Import StateMap.
-Require Import Imp.
+From Stdlib Require Import Arith ZArith Psatz Bool String List Program.Equality.
+From IncLogic Require Import Imp Sequences.
 
-(**
-   We give a semantic interpretation to the statements [Hoare P c Q]
-   of Hoare logic.  The interpretation is the relation [triple P c Q]
-   defined below in terms of IMP's natural semantics
-   (the relation [cexec s c s']).
-*)
+Local Open Scope string_scope.
+Local Open Scope Z_scope.
+Local Open Scope com_scope.
 
-Definition hoare_triple
-           (P : Assertion) (c : com) (s: Signal) (Q : Assertion) : Prop :=
-  forall st st',
-     st =[ c ]=> s: st' ->
-     P st ->
-     Q st'.
 
-Notation "{{ P }} c {{ ε ↑ Q }}" :=
-(hoare_triple P c ε Q) (at level 90, c custom com at level 99): inclogic_spec_scope.
+Definition swap_xy :=
+    ASSIGN "t" (VAR "x");; ASSIGN "x" (VAR "y");; ASSIGN "y" (VAR "t").
 
-Theorem hoare_post_true : forall (P Q : Assertion) s c,
-  (forall st, Q st) ->
-  {{ P }} c {{ s ↑ Q }}.
+
+Lemma swap_xy_correct:
+  forall s, exists s',
+  star red (swap_xy, s) (SKIP, s') /\ s' "x" = s "y" /\ s' "y" = s "x".
 Proof.
-  unfold hoare_triple. intros. apply H.
+  intros. econstructor; split.
+- eapply star_step. apply red_seq_step. apply red_assign.
+  eapply star_step. apply red_seq_done.
+  eapply star_step. apply red_seq_step. apply red_assign.
+  eapply star_step. apply red_seq_done.
+  eapply star_step. apply red_assign.
+  apply star_refl.
+- unfold update; cbn. auto.
 Qed.
 
-Theorem hoare_pre_false : forall (P Q : Assertion) c s,
-  (forall st, ~ (P st)) ->
-  {{ P }} c {{ s ↑ Q }}.
+
+Definition slow_add :=
+  WHILE (LESSEQUAL (CONST 1) (VAR "x")) DO
+        (ASSIGN "x" (MINUS (VAR "x") (CONST 1)) ;;
+         ASSIGN "y" (PLUS  (VAR "y") (CONST 1))) END.
+
+Lemma slow_add_correct:
+  forall s,
+  s "x" >= 0 ->
+  exists s', star red (slow_add, s) (SKIP, s') /\ s' "y" = s "y" + s "x".
 Proof.
-  unfold hoare_triple.
+Admitted.
+
+Definition assertion : Type := store -> Prop.
+
+Definition postassertion : Type := result -> Prop.
+
+Definition aand (P Q: assertion) : assertion :=
+  fun s => P s /\ Q s.
+
+Definition aor (P Q: assertion) : assertion :=
+  fun s => P s \/ Q s.
+
+(** The assertion "arithmetic expression [a] evaluates to value [v]". *)
+
+Definition aequal (a: aexp) (v: Z) : assertion :=
+  fun s => aeval a s = v.
+
+Definition atrue (b: bexp) : assertion :=
+  fun s => beval b s = true.
+
+Definition afalse (b: bexp) : assertion :=
+  fun s => beval b s = false.
+
+(** The assertion written "[ P[x <- a] ]" in the literature.
+    Substituting [a] for [x] in [P] amounts to evaluating [P] in
+    stores where the variable [x] is equal to the value of expression [a]. *)
+
+Definition aupdate (x: ident) (a: aexp) (P: assertion) : assertion :=
+  fun s => P (update x (aeval a s) s).
+
+Notation "P [ x ↦ a ]" := (aupdate x a P) (at level 10).
+
+Example aupdate_example: 
+  (aequal (VAR "y") 5 [ "y" ↦ (PLUS (VAR "y") (CONST 2)) ])
+  (fun _ => 3).
+Proof. cbv. reflexivity. Qed.
+
+(** Pointwise implication.  Unlike conjunction and disjunction, this is
+    not a predicate over the store, just a Coq proposition. *)
+
+Definition aimp (P Q: assertion) : Prop :=
+  forall s, P s -> Q s.
+
+(** A few notations to improve legibility. *)
+
+Notation "P -->> Q" := (aimp P Q) (at level 95, no associativity).
+Notation "P //\\ Q" := (aand P Q) (at level 80, right associativity).
+Notation "P \\// Q" := (aor P Q) (at level 75, right associativity).
+
+
+(** The rules of weak Hoare logic *)
+
+(** Here are the base rules for Hoare logic.
+    They define a relation [Hoare P c Q], where
+-   [P] is the precondition, assumed to hold "before" executing [c];
+-   [c] is the program or program fragment we reason about;
+-   [Q] is the postcondition, guaranteed to hold "after" executing [c].
+
+  This is a "weak" logic, meaning that it does not guarantee termination
+  of the command [c].  What is guaranteed is that if [c] terminates,
+  then its final store satisfies postcondition [Q]. *)
+
+Inductive Hoare: assertion -> com -> assertion -> Prop :=
+| Hoare_skip: forall P,
+  (* ------------------ *)
+  Hoare P SKIP P
+| Hoare_assign: forall P x a,
+  (* ------------------------------ *)
+    Hoare (aupdate x a P) (ASSIGN x a) P
+| Hoare_seq: forall P Q R c1 c2,
+    Hoare P c1 Q ->
+    Hoare Q c2 R ->
+    (* ------------------ *)
+    Hoare P (c1 ;; c2) R
+| Hoare_choice: forall P Q c1 c2,
+    Hoare P c1 Q ->
+    Hoare P c2 Q ->
+    (* ---------------------- *)
+    Hoare P (c1 ⊕ c2) Q
+| Hoare_consequence: forall P Q P' Q' c,
+    Hoare P c Q ->
+    P' -->> P ->
+    Q -->> Q' ->
+    (* -------------*)
+    Hoare P' c Q'
+| Hoare_cstar: forall INV c, 
+    Hoare INV c INV ->
+    (* ------------------ *)
+    Hoare INV (CSTAR c) INV.
+
+Reserved Notation "'hoare' p '<<' c '>>' q"
+  (at level 40, p at level 39, c at level 99, q at level 39).
+
+Inductive HoareRes: assertion -> com -> postassertion -> Prop :=
+| Hoare_skip_r: forall P,
+  (* ------------------ *)
+  hoare P << SKIP >> P
+| Hoare_assign_r: forall P x a,
+  (* ------------------------------ *)
+    hoare (aupdate x a P) << ASSIGN x a >> P
+| Hoare_seq_ok: forall P Q R c1 c2,
+    hoare P << c1 >> Q ->
+    hoare Q << c2 >> R ->
+    (* ------------------ *)
+    hoare P << (c1 ;; c2) >> R
+| Hoare_seq_err: forall P c1 c2,
+    HoareRes P c1 (fun r => match r with RError => True | _ => False end) ->
+    (* ------------------ *)
+    HoareRes P (c1 ;; c2) (fun r => match r with RError => True | _ => False end)
+| Hoare_consequence_res: forall P Q P' Q' c,
+    hoare P << c >> Q ->
+    P' -->> P ->
+    Q -->> Q' ->
+    (* -------------*)
+    hoare P' << c >> Q'
+| Hoare_choice_res: forall P Q c1 c2,
+    hoare P << c1 >> Q ->
+    hoare P << c2 >> Q ->
+    (* ---------------------- *)
+    hoare P << c1 ⊕ c2 >> Q
+| Hoare_cstar_ress: forall INV c, 
+    hoare INV << c >> INV ->
+    (* ------------------ *)
+    hoare INV << CSTAR c >> INV
+where "'hoare' p '<<' c '>>' q" :=
+  (HoareRes p c (fun r => match r with
+                          | RNormal s => q s
+                          | RError => False
+                          end)).
+
+
+Lemma Hoare_consequence_pre: forall P P' Q c,
+      hoare P << c >> Q ->
+      P' -->> P ->
+      hoare P' << c >> Q.
+Proof.
+  intros. apply Hoare_consequence_res with (P := P) (Q := Q); unfold aimp; auto.
+Qed.
+
+Lemma Hoare_consequence_post: forall P Q Q' c,
+      hoare P << c >> Q ->
+      Q -->> Q' ->
+      hoare P << c >> Q'.
+Proof.
+  intros. apply Hoare_consequence_res with (P := P) (Q := Q); unfold aimp; auto.
+Qed.
+
+Example Hoare_swap_xy: forall m n,
+  hoare (aequal (VAR "x") m //\\ aequal (VAR "y") n)
+        << swap_xy >>
+        (aequal (VAR "x") n //\\ aequal (VAR "y") m).
+Proof.
   intros.
-  apply H in H1. destruct H1.
+  eapply Hoare_consequence_pre.
+- unfold swap_xy. eapply Hoare_seq_ok. apply Hoare_assign_r.
+  eapply Hoare_seq_ok. apply Hoare_assign_r. apply Hoare_assign_r.
+- unfold aequal, aupdate, aand, aimp; cbn. tauto.
 Qed.
 
-Theorem hoare_skip : forall P s,
-     {{ P }} skip {{ s ↑ P }}.
+(** * Soundness of Hoare logic *)
+
+(** We give a semantic interpretation to the statements [Hoare P c Q]
+    of Hoare logic.  The interpretation is the relation [triple P c Q]
+    defined below in terms of IMP's natural semantics
+    (the relation [cexec s c s']). *)
+
+Definition triple (P: assertion) (c: com) (Q: assertion) : Prop :=
+  forall s r, cexec s c r -> P s -> (exists s', r = RNormal s' /\ Q s').
+
+Notation "{{ P }} c {{ Q }}" := (triple P c Q) (at level 90, c at next level).
+
+Lemma triple_skip: forall P,
+     {{P}} SKIP {{P}}.
 Proof.
-  intros P s st st' H HP.
-  inversion H; subst; assumption.
+  unfold triple; intros. exists s. inversion H; subst. auto.
 Qed.
 
-Theorem hoare_seq : forall P Q R c1 c2 e,
-     {{ Q }} c2 {{ e ↑ R }} ->
-     {{ P }} c1 {{ ok ↑ Q }} ->
-     {{ P }} c1; c2 {{ e ↑ R }}.
+
+Lemma triple_assign: forall P x a,
+      {{aupdate x a P}} ASSIGN x a {{P}}.
 Proof.
-  unfold hoare_triple.
-  intros P Q R c1 c2 e H1 H2 st st'' H12 Pre.
-  specialize (H1 st st'').
-  
-  (* specialize (H2 st st''). *)
-  
-  (* inversion H12; subst.
-  - specialize (H1 st'0 st').
-    apply H1.
-    assumption.
-    specialize (H2 st st'0).
-    eapply H2; 
-    assumption.
-  - specialize (H1 st st').
-    specialize (H2 st st'). *)
-    
-Admitted. *)
+  unfold triple, aupdate; intros P x a s r EXEC PRE.
+  inversion EXEC; subst.
+  eexists. split; [ reflexivity | exact PRE ].
+Qed.
+
+Lemma triple_seq: forall P Q R c1 c2,
+      {{P}} c1 {{Q}} ->
+      {{Q}} c2 {{R}} ->
+      {{P}} c1;;c2 {{R}}.
+Proof.
+  unfold triple; intros P Q R c1 c2 H1 H2 s r EXEC PRE.
+  inversion EXEC; subst.
+  - (* cexec_seq: c1 normal, c2 normal *)
+    match goal with
+    | E1 : cexec s c1 (RNormal ?s'),
+      E2 : cexec ?s' c2 (RNormal ?s'') |- _ =>
+      destruct (H1 s (RNormal s') E1 PRE) as (sx & EQ1 & QSx);
+      inversion EQ1; subst sx;
+      destruct (H2 s' (RNormal s'') E2 QSx) as (sy & EQ2 & RSy);
+      inversion EQ2; subst sy;
+      exists s''; split; [ reflexivity | exact RSy ]
+    end.
+  - (* cexec_seq_error: c1 errors *)
+    match goal with
+    | E1 : cexec s c1 RError |- _ =>
+      destruct (H1 s RError E1 PRE) as (? & EQ & _); discriminate
+    end.
+  - (* cexec_seq_error_right: c1 normal, c2 errors *)
+    match goal with
+    | E1 : cexec s c1 (RNormal ?s'),
+      E2 : cexec ?s' c2 RError |- _ =>
+      destruct (H1 s (RNormal s') E1 PRE) as (sx & EQ1 & QSx);
+      inversion EQ1; subst sx;
+      destruct (H2 s' RError E2 QSx) as (? & EQ & _); discriminate
+    end.
+Qed.
+
+Lemma triple_ifthenelse: forall P Q b c1 c2,
+      {{atrue b //\\ P}} c1 {{Q}} ->
+      {{afalse b //\\ P}} c2 {{Q}} ->
+      {{P}} IF b THEN c1 ELSE c2 END {{Q}}.
+Proof.
+  unfold triple, aand, atrue, afalse.
+  intros P Q b c1 c2 H1 H2 s r EXEC PRE.
+  inversion EXEC; subst.
+  - (* choice_left: cexec s (ASSUME b ;; c1) r *)
+    match goal with E : cexec s (ASSUME b ;; c1) r |- _ => inversion E; subst end.
+    + (* SEQ normal *)
+      match goal with EA : cexec s (ASSUME b) _ |- _ => inversion EA; subst end.
+      eapply H1; eauto.
+    + (* SEQ error left: ASSUME b errors — impossible *)
+      match goal with EA : cexec s (ASSUME b) RError |- _ => inversion EA end.
+    + (* SEQ error right *)
+      match goal with EA : cexec s (ASSUME b) _ |- _ => inversion EA; subst end.
+      eapply H1; eauto.
+  - (* choice_right: cexec s (ASSUME (NOT b) ;; c2) r *)
+    match goal with E : cexec s (ASSUME (NOT b) ;; c2) r |- _ => inversion E; subst end.
+    + match goal with EA : cexec s (ASSUME (NOT b)) _ |- _ => inversion EA; subst end.
+      eapply H2; eauto.
+      split; [ apply Bool.negb_true_iff; assumption | exact PRE ].
+    + match goal with EA : cexec s (ASSUME (NOT b)) RError |- _ => inversion EA end.
+    + match goal with EA : cexec s (ASSUME (NOT b)) _ |- _ => inversion EA; subst end.
+      eapply H2; eauto.
+      split; [ apply Bool.negb_true_iff; assumption | exact PRE ].
+Qed.
+
+(** Helper: [P] is preserved across any number of iterations of the loop body
+    [(ASSUME b ;; c)] when [c] preserves [P] under the [b]-true precondition. *)
+Lemma triple_while_invariant: forall P b c s s',
+  {{atrue b //\\ P}} c {{P}} ->
+  star (step_iter (ASSUME b ;; c)) s s' ->
+  P s -> P s'.
+Proof.
+  intros P b c s s' H STAR PS.
+  induction STAR as [ x | x y z STEP STAR' IH ]; [ exact PS | ].
+  apply IH. clear IH.
+  unfold step_iter in STEP. inversion STEP. subst.
+  (* STEP gives:
+       H4 : cexec x (ASSUME b) (RNormal s')
+       H6 : cexec s' c (RNormal y)         (where s' is the intermediate)
+     after inversion of the inner ASSUME we get beval b x = true and s' = x. *)
+  match goal with EA : cexec x (ASSUME b) (RNormal ?sm) |- _ => inversion EA; subst sm end.
+  match goal with EC : cexec x c (RNormal y) |- _ =>
+    destruct (H x (RNormal y) EC) as (sx & EQ & PSx);
+      [ split; assumption | inversion EQ; subst sx; exact PSx ]
+  end.
+Qed.
+
+(** Helper: a [cexec] derivation for a [SEQ] command can be decomposed into
+    its three possible shapes. *)
+Lemma cexec_seq_inv:
+  forall c1 c2 s r,
+    cexec s (c1 ;; c2) r ->
+    (exists sm sf, cexec s c1 (RNormal sm) /\ cexec sm c2 (RNormal sf) /\ r = RNormal sf)
+    \/ (cexec s c1 RError /\ r = RError)
+    \/ (exists sm, cexec s c1 (RNormal sm) /\ cexec sm c2 RError /\ r = RError).
+Proof.
+  intros c1 c2 s r EXEC.
+  inversion EXEC; subst.
+  - left. eauto.
+  - right. left. auto.
+  - right. right. eauto.
+Qed.
+
+Lemma triple_while: forall P b c,
+      {{atrue b //\\ P}} c {{P}} ->
+      {{P}} WHILE b DO c END {{afalse b //\\ P}}.
+Proof.
+  unfold triple, aand, atrue, afalse.
+  intros P b c H s r EXEC PRE.
+  (* WHILE b DO c END = ((ASSUME b ;; c) ★) ;; ASSUME (NOT b) *)
+  apply cexec_seq_inv in EXEC.
+  destruct EXEC as
+    [ (sm & sf & EI & EA & ->)
+    | [ (EI & ->) | (sm & EI & EA & ->) ] ].
+  - (* SEQ normal *)
+    apply cexec_cstar_iff_star in EI.
+    assert (PSm : P sm) by (eapply triple_while_invariant; eauto).
+    (* From EA : cexec sm (ASSUME (NOT b)) (RNormal sf) extract: sm = sf, beval (NOT b) sm = true *)
+    inversion EA as [ | | | | ?se ?bv HBeval HEq | | | | | | | | | ]; subst.
+    exists sf; split;
+      [ reflexivity
+      | split; [ apply Bool.negb_true_iff; exact HBeval | exact PSm ] ].
+  - (* SEQ error left: iterated body errors *)
+    apply cexec_cstar_err_iff in EI.
+    destruct EI as (sm & STAR & ERR).
+    assert (PSm : P sm) by (eapply triple_while_invariant; eauto).
+    apply cexec_seq_inv in ERR.
+    destruct ERR as
+      [ (sm1 & sf1 & _ & _ & EQbad)
+      | [ (EA & _) | (sx & EA & EC & _) ] ].
+    + (* normal yields RNormal, can't equal RError *)
+      discriminate EQbad.
+    + (* ASSUME b errors: impossible *)
+      inversion EA.
+    + (* ASSUME b ok, c errors: contradicts H. EA : cexec sm (ASSUME b) (RNormal sx) *)
+      inversion EA; subst sx.   (* substitute sx := sm only *)
+      destruct (H sm RError EC) as (? & EQc & _);
+        [ split; assumption | discriminate ].
+  - (* SEQ error right: ASSUME (NOT b) errors. Impossible. *)
+    inversion EA.
+Qed.
+
+Lemma triple_consequence: forall P Q P' Q' c,
+      {{P}} c {{Q}} ->
+      P' -->> P ->
+      Q -->> Q' ->
+      {{P'}} c {{Q'}}.
+Proof.
+  unfold triple, aimp; intros P Q P' Q' c HT P'P QQ' s r EXEC PRE.
+  destruct (HT s r EXEC (P'P s PRE)) as (s' & EQ & QSx).
+  exists s'. split; [ exact EQ | apply QQ', QSx ].
+Qed.
+
+(** Strong Hoare triples *)
+
+Definition Triple (P: assertion) (c: com) (Q: assertion) :=
+  forall s, P s -> exists s', cexec s c (RNormal s') /\ Q s'.
+
+Notation "{{{ P }}} c {{{ Q }}}" := (Triple P c Q) (at level 90, c at next level).
